Add parameters to reactions

Main.lean
@@ -32,7 +32,7 @@ lf {
           let c ← getState count
           setOutput out c
           setState count (c + 1)
-          monadLift <| IO.println s!"{c}"
+          IO.println s!"{c}"
         }
       }
     ]
@@ -42,3 +42,32 @@ def main : IO Unit := do
   let exec := LF.executable (← Time.now)
   let topo : Array (Network.ReactionID LF.network) := #[⟨.nil, ⟨0, by simp⟩⟩]
   exec.run topo 0
+
+
+
+
+
+
+
+
+#synth MonadLift IO (
+  ReactionM (Interface.Scheme.restrict (Network.Graph.reactionInputScheme LF.graph .Main) LF.Main.Reaction0.PortSource)
+    (Interface.Scheme.restrict (Network.Graph.reactionOutputScheme LF.graph .Main) LF.Main.Reaction0.PortEffect)
+    (Interface.Scheme.restrict (Network.Graph.interface LF.graph .Main Reactor.InterfaceKind.actions) LF.Main.Reaction0.ActionSource)
+    (Interface.Scheme.restrict (Network.Graph.interface LF.graph .Main Reactor.InterfaceKind.actions) LF.Main.Reaction0.ActionEffect)
+    (Network.Graph.interface LF.graph .Main Reactor.InterfaceKind.state)
+)
+
+
+
+structure In : Type
+structure Out : Type
+
+def ThingM (n₁ n₂ : Nat) (α : Type) := In → IO (α × Out)
+
+instance : Monad (ThingM n₁ n₂) := sorry
+instance : MonadLift IO (ThingM n₁ n₂) := sorry
+
+example : ThingM 1 2 Nat := do
+  IO.println ""
+  return 2
