Runtime/Reaction.lean
@@ -13,10 +13,11 @@ instance : Ord (Reaction.Event σAction time) where
 namespace ReactionM
 open Reaction
 
-structure Input (σPortSource σActionSource σState : Interface.Scheme) where
+structure Input (σPortSource σActionSource σState σParam : Interface.Scheme) where
   ports          : Interface? σPortSource
   actions        : Interface? σActionSource
   state          : Interface σState
+  params         : Interface σParam
   tag            : Tag
   physicalOffset : Duration
 
@@ -25,22 +26,23 @@ structure Output (σPortEffect σActionEffect σState : Interface.Scheme) (min :
   state  : Interface σState
   events : SortedArray (Event σActionEffect min) := #[]#
 
-abbrev _root_.ReactionT (σPortSource σPortEffect σActionSource σActionEffect σState : Interface.Scheme) (m : Type → Type) (α : Type) := 
-  (input : Input σPortSource σActionSource σState) → m (Output σPortEffect σActionEffect σState input.tag.time × α)
+abbrev _root_.ReactionT (σPortSource σPortEffect σActionSource σActionEffect σState σParam : Interface.Scheme) (m : Type → Type) (α : Type) := 
+  (input : Input σPortSource σActionSource σState σParam) → m (Output σPortEffect σActionEffect σState input.tag.time × α)
 
-abbrev _root_.ReactionM (σPortSource σPortEffect σActionSource σActionEffect σState : Interface.Scheme) := ReactionT σPortSource σPortEffect σActionSource σActionEffect σState IO
+abbrev _root_.ReactionM (σPortSource σPortEffect σActionSource σActionEffect σState σParam : Interface.Scheme) := 
+  ReactionT σPortSource σPortEffect σActionSource σActionEffect σState σParam IO
 
-variable {σInput σOutput σAction σPortSource σPortEffect σActionSource σActionEffect σState : Interface.Scheme} 
+variable {σInput σOutput σAction σPortSource σPortEffect σActionSource σActionEffect σState σParam : Interface.Scheme} 
 
 def Output.merge (o₁ o₂ : ReactionM.Output σPortEffect σActionEffect σState time) : Output σPortEffect σActionEffect σState time where
   ports  := o₁.ports.merge o₂.ports
   state  := o₂.state
   events := o₁.events.merge o₂.events
 
-def Input.noop (input : ReactionM.Input σPortSource σActionSource σState) : Output σPortEffect σActionEffect σState input.tag.time where 
+def Input.noop (input : ReactionM.Input σPortSource σActionSource σState σParam) : Output σPortEffect σActionEffect σState input.tag.time where 
   state := input.state 
 
-instance : Monad (ReactionM σPortSource σPortEffect σActionSource σActionEffect σState) where
+instance : Monad (ReactionM σPortSource σPortEffect σActionSource σActionEffect σState σParam) where
   pure a input := do
     let output := input.noop
     return (output, a)
@@ -59,43 +61,46 @@ instance : Monad (ReactionM σPortSource σPortEffect σActionSource σActionEff
     let output := output₁.merge output₂
     return (output, b)
 
-instance : MonadLift IO (ReactionM σPortSource σPortEffect σActionSource σActionEffect σState) where
+instance : MonadLift IO (ReactionM σPortSource σPortEffect σActionSource σActionEffect σState σParam) where
   monadLift io input world := 
     match io world with 
     | .error e world' => .error e world'
     | .ok    a world' => .ok (input.noop, a) world'
 
-def getInput (port : σPortSource.vars) : ReactionM σPortSource σPortEffect σActionSource σActionEffect σState (Option $ σPortSource.type port) :=
+def getInput (port : σPortSource.vars) : ReactionM σPortSource σPortEffect σActionSource σActionEffect σState σParam (Option $ σPortSource.type port) :=
   fun input => return (input.noop, input.ports port)
 
-def getState (stv : σState.vars) : ReactionM σPortSource σPortEffect σActionSource σActionEffect σState (σState.type stv) :=
+def getState (stv : σState.vars) : ReactionM σPortSource σPortEffect σActionSource σActionEffect σState σParam (σState.type stv) :=
   fun input => return (input.noop, input.state stv)
 
-def getAction (action : σActionSource.vars) : ReactionM σPortSource σPortEffect σActionSource σActionEffect σState (Option $ σActionSource.type action) :=
+def getAction (action : σActionSource.vars) : ReactionM σPortSource σPortEffect σActionSource σActionEffect σState σParam (Option $ σActionSource.type action) :=
   fun input => return (input.noop, input.actions action)
 
-def getTag : ReactionM σPortSource σPortEffect σActionSource σActionEffect σState Tag := 
+def getParam (param : σParam.vars) : ReactionM σPortSource σPortEffect σActionSource σActionEffect σState σParam (σParam.type param) :=
+  fun input => return (input.noop, input.params param)
+
+def getTag : ReactionM σPortSource σPortEffect σActionSource σActionEffect σState σParam Tag := 
   fun input => return (input.noop, input.tag)
 
-def getLogicalTime : ReactionM σPortSource σPortEffect σActionSource σActionEffect σState Time := 
+def getLogicalTime : ReactionM σPortSource σPortEffect σActionSource σActionEffect σState σParam Time := 
   return (← getTag).time
 
-def getPhysicalTime : ReactionM σPortSource σPortEffect σActionSource σActionEffect σState Time :=
+def getPhysicalTime : ReactionM σPortSource σPortEffect σActionSource σActionEffect σState σParam Time :=
   fun input => return (input.noop, (← Time.now) - input.physicalOffset)
 
-def setOutput (port : σPortEffect.vars) (v : σPortEffect.type port) : ReactionM σPortSource σPortEffect σActionSource σActionEffect σState Unit :=
+def setOutput (port : σPortEffect.vars) (v : σPortEffect.type port) : ReactionM σPortSource σPortEffect σActionSource σActionEffect σState σParam Unit :=
   fun input => 
     let ports := fun p => if h : p = port then some (h ▸ v) else none
     let output := { ports := ports, state := input.state }
     return (output, ())
 
-def setState (stv : σState.vars) (v : σState.type stv) : ReactionM σPortSource σPortEffect σActionSource σActionEffect σState Unit :=
+def setState (stv : σState.vars) (v : σState.type stv) : ReactionM σPortSource σPortEffect σActionSource σActionEffect σState σParam Unit :=
   fun input =>
     let state := fun s => if h : s = stv then h ▸ v else input.state s
     let output := { state := state }
     return (output, ())
 
-def schedule (action : σActionEffect.vars) (delay : Duration) (v : σActionEffect.type action) : ReactionM σPortSource σPortEffect σActionSource σActionEffect σState Unit := 
+def schedule (action : σActionEffect.vars) (delay : Duration) (v : σActionEffect.type action) : ReactionM σPortSource σPortEffect σActionSource σActionEffect σState σParam Unit := 
   fun input => 
     let time := input.tag.time.advance delay
     let event : Event σActionEffect input.tag.time := { action := action, time := time, value := v }
@@ -114,7 +119,7 @@ inductive Trigger (Port Action Timer : Type)
   | timer (t : Timer)
 
 open Reaction in
-structure _root_.Reaction (σInput σOutput σAction σState : Interface.Scheme) (TimerNames : Type) where
+structure _root_.Reaction (σInput σOutput σAction σState σParam : Interface.Scheme) (TimerNames : Type) where
   portSources : Type
   portEffects : Type 
   actionSources : Type
@@ -128,16 +133,25 @@ structure _root_.Reaction (σInput σOutput σAction σState : Interface.Scheme)
   [portEffectsInjCoe : InjectiveCoe portEffects σOutput.vars]
   [actionSourcesInjCoe : InjectiveCoe actionSources σAction.vars]
   [actionEffectsInjCoe : InjectiveCoe actionEffects σAction.vars]
-  body : ReactionM (σInput.restrict portSources) (σOutput.restrict portEffects) (σAction.restrict actionSources) (σAction.restrict actionEffects) σState Unit
+  body : ReactionM (σInput.restrict portSources) (σOutput.restrict portEffects) (σAction.restrict actionSources) (σAction.restrict actionEffects) σState σParam Unit
 
 open Reaction in
 attribute [instance] portSourcesDecEq portEffectsDecEq actionSourcesDecEq actionEffectsDecEq portSourcesInjCoe portEffectsInjCoe actionSourcesInjCoe actionEffectsInjCoe
 
-abbrev outputType (rcn : Reaction σInput σOutput σAction σState TimerNames) :=
+abbrev outputType (rcn : Reaction σInput σOutput σAction σState σParam TimerNames) :=
   ReactionM.Output (σOutput.restrict rcn.portEffects) (σAction.restrict rcn.actionEffects) σState 
 
-def run (rcn : Reaction σInput σOutput σAction σState TimerNames) (inputs : Interface? σInput) (actions : Interface? σAction) (state : Interface σState) (tag : Tag) (physicalOffset : Duration) : IO (rcn.outputType tag.time) := do
-  let ⟨output, _⟩ ← rcn.body { ports := (inputs ·), actions := (actions ·), state := state, tag := tag, physicalOffset := physicalOffset }
+def run 
+  (rcn : Reaction σInput σOutput σAction σState σParam TimerNames) 
+  (inputs : Interface? σInput) (actions : Interface? σAction) 
+  (state : Interface σState) (params : Interface σParam) 
+  (tag : Tag) (physicalOffset : Duration) : 
+  IO (rcn.outputType tag.time) := do
+  let ⟨output, _⟩ ← rcn.body { 
+    ports := (inputs ·), actions := (actions ·), 
+    state := state, params := params, 
+    tag := tag, physicalOffset := physicalOffset 
+  }
   return output
 
 end Reaction
